ocaml/fstar-lib/generated/FStar_SMTEncoding_SolverState.ml
@@ -18,44 +18,60 @@ type decls_at_level =
   given_decl_names: decl_name_set ;
   all_decls_at_level_rev: FStar_SMTEncoding_Term.decl Prims.list ;
   given_decls_rev: FStar_SMTEncoding_Term.decl Prims.list ;
-  to_flush_rev: FStar_SMTEncoding_Term.decl Prims.list }
+  to_flush_rev: FStar_SMTEncoding_Term.decl Prims.list ;
+  named_assumptions:
+    FStar_SMTEncoding_Term.assumption FStar_Compiler_Util.psmap }
 let (__proj__Mkdecls_at_level__item__pruning_state :
   decls_at_level -> FStar_SMTEncoding_Pruning.pruning_state) =
   fun projectee ->
     match projectee with
     | { pruning_state; given_decl_names; all_decls_at_level_rev;
-        given_decls_rev; to_flush_rev;_} -> pruning_state
+        given_decls_rev; to_flush_rev; named_assumptions;_} -> pruning_state
 let (__proj__Mkdecls_at_level__item__given_decl_names :
   decls_at_level -> decl_name_set) =
   fun projectee ->
     match projectee with
     | { pruning_state; given_decl_names; all_decls_at_level_rev;
-        given_decls_rev; to_flush_rev;_} -> given_decl_names
+        given_decls_rev; to_flush_rev; named_assumptions;_} ->
+        given_decl_names
 let (__proj__Mkdecls_at_level__item__all_decls_at_level_rev :
   decls_at_level -> FStar_SMTEncoding_Term.decl Prims.list) =
   fun projectee ->
     match projectee with
     | { pruning_state; given_decl_names; all_decls_at_level_rev;
-        given_decls_rev; to_flush_rev;_} -> all_decls_at_level_rev
+        given_decls_rev; to_flush_rev; named_assumptions;_} ->
+        all_decls_at_level_rev
 let (__proj__Mkdecls_at_level__item__given_decls_rev :
   decls_at_level -> FStar_SMTEncoding_Term.decl Prims.list) =
   fun projectee ->
     match projectee with
     | { pruning_state; given_decl_names; all_decls_at_level_rev;
-        given_decls_rev; to_flush_rev;_} -> given_decls_rev
+        given_decls_rev; to_flush_rev; named_assumptions;_} ->
+        given_decls_rev
 let (__proj__Mkdecls_at_level__item__to_flush_rev :
   decls_at_level -> FStar_SMTEncoding_Term.decl Prims.list) =
   fun projectee ->
     match projectee with
     | { pruning_state; given_decl_names; all_decls_at_level_rev;
-        given_decls_rev; to_flush_rev;_} -> to_flush_rev
+        given_decls_rev; to_flush_rev; named_assumptions;_} -> to_flush_rev
+let (__proj__Mkdecls_at_level__item__named_assumptions :
+  decls_at_level ->
+    FStar_SMTEncoding_Term.assumption FStar_Compiler_Util.psmap)
+  =
+  fun projectee ->
+    match projectee with
+    | { pruning_state; given_decl_names; all_decls_at_level_rev;
+        given_decls_rev; to_flush_rev; named_assumptions;_} ->
+        named_assumptions
 let (init_given_decls_at_level : decls_at_level) =
+  let uu___ = FStar_Compiler_Util.psmap_empty () in
   {
     pruning_state = FStar_SMTEncoding_Pruning.init;
     given_decl_names = empty_decl_names;
     all_decls_at_level_rev = [];
     given_decls_rev = [];
-    to_flush_rev = []
+    to_flush_rev = [];
+    named_assumptions = uu___
   }
 type solver_state =
   {
@@ -156,7 +172,8 @@ let (push : solver_state -> solver_state) =
             given_decls_rev = [];
             to_flush_rev =
               [FStar_SMTEncoding_Term.Push
-                 (FStar_Compiler_List.length s.levels)]
+                 (FStar_Compiler_List.length s.levels)];
+            named_assumptions = (hd.named_assumptions)
           } in
         let s1 =
           {
@@ -193,35 +210,75 @@ let (pop : solver_state -> solver_state) =
                 using_facts_from = (s.using_facts_from)
               } in
           debug "pop" s s1; s1))
-let (reset :
+let (filter_using_facts_from :
   using_facts_from_setting FStar_Pervasives_Native.option ->
-    solver_state -> solver_state)
+    FStar_SMTEncoding_Term.assumption FStar_Compiler_Util.psmap ->
+      solver_state ->
+        FStar_SMTEncoding_Term.decl Prims.list ->
+          FStar_SMTEncoding_Term.decl Prims.list)
   =
   fun using_facts_from ->
-    fun s ->
-      let levels =
-        FStar_Compiler_List.map
-          (fun level ->
-             {
-               pruning_state = (level.pruning_state);
-               given_decl_names = (level.given_decl_names);
-               all_decls_at_level_rev = (level.all_decls_at_level_rev);
-               given_decls_rev = [];
-               to_flush_rev =
-                 (FStar_List_Tot_Base.op_At level.to_flush_rev
-                    level.given_decls_rev)
-             }) s.levels in
-      let using_facts_from1 =
-        match using_facts_from with
-        | FStar_Pervasives_Native.Some u -> FStar_Pervasives_Native.Some u
-        | FStar_Pervasives_Native.None -> s.using_facts_from in
-      let s1 =
-        {
-          levels;
-          pending_flushes_rev = [];
-          using_facts_from = using_facts_from1
-        } in
-      debug "reset" s s1; s1
+    fun named_assumptions ->
+      fun s ->
+        fun ds ->
+          match using_facts_from with
+          | FStar_Pervasives_Native.None -> ds
+          | FStar_Pervasives_Native.Some (([], true)::[]) -> ds
+          | FStar_Pervasives_Native.Some using_facts_from1 ->
+              let keep_assumption a =
+                match a.FStar_SMTEncoding_Term.assumption_fact_ids with
+                | [] -> true
+                | uu___ ->
+                    FStar_Compiler_Util.for_some
+                      (fun uu___1 ->
+                         match uu___1 with
+                         | FStar_SMTEncoding_Term.Name lid ->
+                             FStar_TypeChecker_Env.should_enc_lid
+                               using_facts_from1 lid
+                         | uu___2 -> false)
+                      a.FStar_SMTEncoding_Term.assumption_fact_ids in
+              let already_given_map =
+                FStar_Compiler_Util.smap_create (Prims.of_int (1000)) in
+              let add_assumption a =
+                FStar_Compiler_Util.smap_add already_given_map
+                  a.FStar_SMTEncoding_Term.assumption_name true in
+              let already_given a =
+                (let uu___ =
+                   FStar_Compiler_Util.smap_try_find already_given_map
+                     a.FStar_SMTEncoding_Term.assumption_name in
+                 FStar_Pervasives_Native.uu___is_Some uu___) ||
+                  (FStar_Compiler_Util.for_some
+                     (fun level ->
+                        decl_names_contains
+                          a.FStar_SMTEncoding_Term.assumption_name
+                          level.given_decl_names) s.levels) in
+              let map_decl d =
+                match d with
+                | FStar_SMTEncoding_Term.Assume a ->
+                    let uu___ =
+                      (keep_assumption a) &&
+                        (let uu___1 = already_given a in
+                         Prims.op_Negation uu___1) in
+                    if uu___ then (add_assumption a; [d]) else []
+                | FStar_SMTEncoding_Term.RetainAssumptions names ->
+                    let assumptions =
+                      FStar_Compiler_List.collect
+                        (fun name ->
+                           let uu___ =
+                             FStar_Compiler_Util.psmap_try_find
+                               named_assumptions name in
+                           match uu___ with
+                           | FStar_Pervasives_Native.None -> []
+                           | FStar_Pervasives_Native.Some a ->
+                               let uu___1 = already_given a in
+                               if uu___1
+                               then []
+                               else
+                                 (add_assumption a;
+                                  [FStar_SMTEncoding_Term.Assume a])) names in
+                    assumptions
+                | uu___ -> [d] in
+              let ds1 = FStar_Compiler_List.collect map_decl ds in ds1
 let rec (flatten :
   FStar_SMTEncoding_Term.decl -> FStar_SMTEncoding_Term.decl Prims.list) =
   fun d ->
@@ -229,6 +286,21 @@ let rec (flatten :
     | FStar_SMTEncoding_Term.Module (uu___, ds) ->
         FStar_Compiler_List.collect flatten ds
     | uu___ -> [d]
+let (add_named_assumptions :
+  FStar_SMTEncoding_Term.assumption FStar_Compiler_Util.psmap ->
+    FStar_SMTEncoding_Term.decl Prims.list ->
+      FStar_SMTEncoding_Term.assumption FStar_Compiler_Util.psmap)
+  =
+  fun named_assumptions ->
+    fun ds ->
+      FStar_Compiler_List.fold_left
+        (fun named_assumptions1 ->
+           fun d ->
+             match d with
+             | FStar_SMTEncoding_Term.Assume a ->
+                 FStar_Compiler_Util.psmap_add named_assumptions1
+                   a.FStar_SMTEncoding_Term.assumption_name a
+             | uu___ -> named_assumptions1) named_assumptions ds
 let (give_now :
   FStar_SMTEncoding_Term.decl Prims.list -> solver_state -> solver_state) =
   fun ds ->
@@ -238,10 +310,15 @@ let (give_now :
         FStar_Compiler_List.partition FStar_SMTEncoding_Term.uu___is_Assume
           decls in
       match uu___ with
-      | (assumptions, rest) ->
-          let uu___1 = peek s in
-          (match uu___1 with
+      | (assumptions, uu___1) ->
+          let uu___2 = peek s in
+          (match uu___2 with
            | (hd, tl) ->
+               let named_assumptions =
+                 add_named_assumptions hd.named_assumptions assumptions in
+               let ds_to_flush =
+                 filter_using_facts_from s.using_facts_from named_assumptions
+                   s decls in
                let given =
                  FStar_Compiler_List.fold_left
                    (fun given1 ->
@@ -249,21 +326,23 @@ let (give_now :
                         match d with
                         | FStar_SMTEncoding_Term.Assume a ->
                             add_name a.FStar_SMTEncoding_Term.assumption_name
-                              given1) hd.given_decl_names assumptions in
+                              given1
+                        | uu___3 -> given1) hd.given_decl_names ds_to_flush in
                let hd1 =
-                 let uu___2 =
+                 let uu___3 =
                    FStar_SMTEncoding_Pruning.add_assumptions assumptions
                      hd.pruning_state in
                  {
-                   pruning_state = uu___2;
+                   pruning_state = uu___3;
                    given_decl_names = given;
                    all_decls_at_level_rev =
                      (FStar_List_Tot_Base.op_At (FStar_Compiler_List.rev ds)
                         hd.all_decls_at_level_rev);
                    given_decls_rev = (hd.given_decls_rev);
                    to_flush_rev =
-                     (FStar_List_Tot_Base.op_At (FStar_Compiler_List.rev ds)
-                        hd.to_flush_rev)
+                     (FStar_List_Tot_Base.op_At
+                        (FStar_Compiler_List.rev ds_to_flush) hd.to_flush_rev);
+                   named_assumptions
                  } in
                {
                  levels = (hd1 :: tl);
@@ -273,6 +352,57 @@ let (give_now :
 let (give :
   FStar_SMTEncoding_Term.decl Prims.list -> solver_state -> solver_state) =
   fun ds -> fun s -> let s1 = give_now ds s in debug "give" s s1; s1
+let (reset_with_new_using_facts_from :
+  using_facts_from_setting FStar_Pervasives_Native.option ->
+    solver_state -> solver_state)
+  =
+  fun using_facts_from ->
+    fun s ->
+      let s_new = init () in
+      let s_new1 =
+        {
+          levels = (s_new.levels);
+          pending_flushes_rev = (s_new.pending_flushes_rev);
+          using_facts_from
+        } in
+      let rec rebuild levels s_new2 =
+        match levels with
+        | last::[] ->
+            give (FStar_Compiler_List.rev last.all_decls_at_level_rev) s_new2
+        | level::levels1 ->
+            let s_new3 = let uu___ = rebuild levels1 s_new2 in push uu___ in
+            give (FStar_Compiler_List.rev level.all_decls_at_level_rev)
+              s_new3 in
+      rebuild s.levels s_new1
+let (reset :
+  using_facts_from_setting FStar_Pervasives_Native.option ->
+    solver_state -> solver_state)
+  =
+  fun using_facts_from ->
+    fun s ->
+      if using_facts_from = s.using_facts_from
+      then
+        let levels =
+          FStar_Compiler_List.map
+            (fun level ->
+               {
+                 pruning_state = (level.pruning_state);
+                 given_decl_names = (level.given_decl_names);
+                 all_decls_at_level_rev = (level.all_decls_at_level_rev);
+                 given_decls_rev = [];
+                 to_flush_rev =
+                   (FStar_List_Tot_Base.op_At level.to_flush_rev
+                      level.given_decls_rev);
+                 named_assumptions = (level.named_assumptions)
+               }) s.levels in
+        let s1 =
+          {
+            levels;
+            pending_flushes_rev = [];
+            using_facts_from = (s.using_facts_from)
+          } in
+        (debug "reset" s s1; s1)
+      else reset_with_new_using_facts_from using_facts_from s
 let (name_of_assumption : FStar_SMTEncoding_Term.decl -> Prims.string) =
   fun d ->
     match d with
@@ -315,7 +445,8 @@ let (flush :
              given_decls_rev =
                (FStar_List_Tot_Base.op_At level.to_flush_rev
                   level.given_decls_rev);
-             to_flush_rev = []
+             to_flush_rev = [];
+             named_assumptions = (level.named_assumptions)
            }) s.levels in
     let s1 =
       {
